Mobius Inversion
$F(n)=\sum_{d|n}f(d)\Rightarrow f(n)=\sum_{d|n}\mu(d)F(\frac{n}{d})$
$F(n)=\sum_{n|d}f(d)\Rightarrow f(n)=\sum_{n|d}\mu(\frac{d}{n})F(d)$
```cpp
int prime[maxn], mu[maxn];
bool heshu[maxn];
void getMu(int n)
{
    mu[1] = 1;
    for (int i = 2; i <= n; ++i)
    {
        if (!heshu[i])
            prime[++prime[0]] = i, mu[i] = -1;
        for (int j = 1; j <= prime[0] && i * prime[j] <= n; ++j)
        {
            heshu[i * prime[j]] = true;
            if (i % prime[j] == 0)
            {
                mu[i * prime[j]] = 0;
                break;
            }
            else
                mu[i * prime[j]] = -mu[i];
        }
    }
}
```